theories/ty_interp_subst_lemmas.v
@@ -6,7 +6,6 @@ Module Type TyInterpLemmas (Import VS : VlSortsFullSig) (Import LWP : LiftWp VS)
 Class TyInterp ty Σ :=
   ty_interp : ty -> envD Σ.
 Notation "⟦ T ⟧" := (ty_interp T).
-Notation "⟦ g ⟧g" := (fmap (M := gmap stamp) ty_interp g).
 
 (* Also appears in Autosubst. *)
 Global Arguments ty_interp {_ _ _} !_ /.
